## Structure constants of the Lie Algebra:
$(0, \0, \0, \e^{ 15 }, \0, \e^{ 13 })$ 

### Symplectic form
 $\omega=e^{ 12 } + e^{ 34 } + e^{ 56 }$

### Derivatives of $3-$forms
$d(e^{ 124 })  = (-1)e^{ 1125 }$

$d(e^{ 126 })  = (-1)e^{ 1123 }$

$d(e^{ 134 })  = (-1)e^{ 1135 }$

$d(e^{ 136 })  = (-1)e^{ 1133 }$

$d(e^{ 145 })  = e^{ 1155 }$

$d(e^{ 146 })  = e^{ 1134 } + (-1)e^{ 1156 }$

$d(e^{ 156 })  = e^{ 1135 }$

$d(e^{ 234 })  = e^{ 1235 }$

$d(e^{ 236 })  = e^{ 1233 }$

$d(e^{ 245 })  = (-1)e^{ 1255 }$

$d(e^{ 246 })  = (-1)e^{ 1234 } + e^{ 1256 }$

$d(e^{ 256 })  = (-1)e^{ 1235 }$

$d(e^{ 345 })  = (-1)e^{ 1355 }$

$d(e^{ 346 })  = (-1)e^{ 1334 } + e^{ 1356 }$

$d(e^{ 356 })  = (-1)e^{ 1335 }$

$d(e^{ 456 })  = e^{ 1345 } + (-1)e^{ 1556 }$

### Derivatives of $2-$forms
$d(e^{ 14 })  = (-1)e^{ 115 }$

$d(e^{ 16 })  = (-1)e^{ 113 }$

$d(e^{ 24 })  = e^{ 125 }$

$d(e^{ 26 })  = e^{ 123 }$

$d(e^{ 34 })  = e^{ 135 }$

$d(e^{ 36 })  = e^{ 133 }$

$d(e^{ 45 })  = (-1)e^{ 155 }$

$d(e^{ 46 })  = (-1)e^{ 134 } + e^{ 156 }$

$d(e^{ 56 })  = (-1)e^{ 135 }$

### $d \Lambda d$ of $3-$forms
$d \Lambda d( e^{ 246 })  = (-2)e^{ 135 }$

\pagebreak

## Structure constants of the Lie Algebra:
$(0, \0, \0, \0, \e^{ 12 }, \e^{ 13 })$ 

### Symplectic form
 $\omega=(-1)e^{ 16 } + e^{ 25 } + e^{ 34 }$

### Derivatives of $3-$forms
$d(e^{ 125 })  = (-1)e^{ 1122 }$

$d(e^{ 126 })  = (-1)e^{ 1123 }$

$d(e^{ 135 })  = e^{ 1123 }$

$d(e^{ 136 })  = (-1)e^{ 1133 }$

$d(e^{ 145 })  = e^{ 1124 }$

$d(e^{ 146 })  = e^{ 1134 }$

$d(e^{ 156 })  = (-1)e^{ 1126 } + e^{ 1135 }$

$d(e^{ 235 })  = (-1)e^{ 1223 }$

$d(e^{ 236 })  = e^{ 1233 }$

$d(e^{ 245 })  = (-1)e^{ 1224 }$

$d(e^{ 246 })  = (-1)e^{ 1234 }$

$d(e^{ 256 })  = e^{ 1226 } + (-1)e^{ 1235 }$

$d(e^{ 345 })  = e^{ 1234 }$

$d(e^{ 346 })  = (-1)e^{ 1334 }$

$d(e^{ 356 })  = (-1)e^{ 1236 } + (-1)e^{ 1335 }$

$d(e^{ 456 })  = (-1)e^{ 1246 } + e^{ 1345 }$

### Derivatives of $2-$forms
$d(e^{ 15 })  = (-1)e^{ 112 }$

$d(e^{ 16 })  = (-1)e^{ 113 }$

$d(e^{ 25 })  = e^{ 122 }$

$d(e^{ 26 })  = e^{ 123 }$

$d(e^{ 35 })  = (-1)e^{ 123 }$

$d(e^{ 36 })  = e^{ 133 }$

$d(e^{ 45 })  = (-1)e^{ 124 }$

$d(e^{ 46 })  = (-1)e^{ 134 }$

$d(e^{ 56 })  = e^{ 126 } + (-1)e^{ 135 }$

### $d \Lambda d$ of $3-$forms
$d \Lambda d( e^{ 456 })  = (-1)e^{ 112 }$

\pagebreak

## Structure constants of the Lie Algebra:
$(0, \e^{ 35 }, \0, \0.5e^{ 15 }, \0, \(-0.5)e^{ 13 })$ 

### Symplectic form
 $\omega=e^{ 12 } + e^{ 34 } + e^{ 56 }$

### Derivatives of $3-$forms
$d(e^{ 123 })  = (-1)e^{ 1335 }$

$d(e^{ 124 })  = (-0.5)e^{ 1125 } + e^{ 1345 }$

$d(e^{ 125 })  = e^{ 1355 }$

$d(e^{ 126 })  = 0.5e^{ 1123 } + (-1)e^{ 1356 }$

$d(e^{ 134 })  = (-0.5)e^{ 1135 }$

$d(e^{ 136 })  = 0.5e^{ 1133 }$

$d(e^{ 145 })  = 0.5e^{ 1155 }$

$d(e^{ 146 })  = (-0.5)e^{ 1134 } + (-0.5)e^{ 1156 }$

$d(e^{ 156 })  = (-0.5)e^{ 1135 }$

$d(e^{ 234 })  = 0.5e^{ 1235 } + (-1)e^{ 3345 }$

$d(e^{ 235 })  = (-1)e^{ 3355 }$

$d(e^{ 236 })  = (-0.5)e^{ 1233 } + e^{ 3356 }$

$d(e^{ 245 })  = (-0.5)e^{ 1255 } + e^{ 3455 }$

$d(e^{ 246 })  = 0.5e^{ 1234 } + 0.5e^{ 1256 } + (-1)e^{ 3456 }$

$d(e^{ 256 })  = 0.5e^{ 1235 } + (-1)e^{ 3556 }$

$d(e^{ 345 })  = (-0.5)e^{ 1355 }$

$d(e^{ 346 })  = 0.5e^{ 1334 } + 0.5e^{ 1356 }$

$d(e^{ 356 })  = 0.5e^{ 1335 }$

$d(e^{ 456 })  = (-0.5)e^{ 1345 } + (-0.5)e^{ 1556 }$

### Derivatives of $2-$forms
$d(e^{ 12 })  = (-1)e^{ 135 }$

$d(e^{ 14 })  = (-0.5)e^{ 115 }$

$d(e^{ 16 })  = 0.5e^{ 113 }$

$d(e^{ 23 })  = e^{ 335 }$

$d(e^{ 24 })  = 0.5e^{ 125 } + (-1)e^{ 345 }$

$d(e^{ 25 })  = (-1)e^{ 355 }$

$d(e^{ 26 })  = (-0.5)e^{ 123 } + e^{ 356 }$

$d(e^{ 34 })  = 0.5e^{ 135 }$

$d(e^{ 36 })  = (-0.5)e^{ 133 }$

$d(e^{ 45 })  = (-0.5)e^{ 155 }$

$d(e^{ 46 })  = 0.5e^{ 134 } + 0.5e^{ 156 }$

$d(e^{ 56 })  = 0.5e^{ 135 }$

### $d \Lambda d$ of $3-$forms
$d \Lambda d( e^{ 246 })  = (-1.5)e^{ 135 }$

\pagebreak

## Structure constants of the Lie Algebra:
$(0, \0, \0, \e^{ 12 }, \e^{ 13 }, \e^{ 23 })$ 

### Symplectic form
 $\omega=2e^{ 16 } + e^{ 25 } + (-1)e^{ 34 }$

### Derivatives of $3-$forms
$d(e^{ 124 })  = (-1)e^{ 1122 }$

$d(e^{ 125 })  = (-1)e^{ 1123 }$

$d(e^{ 126 })  = e^{ 1223 }$

$d(e^{ 134 })  = e^{ 1123 }$

$d(e^{ 135 })  = (-1)e^{ 1133 }$

$d(e^{ 136 })  = (-1)e^{ 1233 }$

$d(e^{ 145 })  = (-1)e^{ 1125 } + e^{ 1134 }$

$d(e^{ 146 })  = (-1)e^{ 1126 } + e^{ 1234 }$

$d(e^{ 156 })  = (-1)e^{ 1136 } + e^{ 1235 }$

$d(e^{ 234 })  = (-1)e^{ 1223 }$

$d(e^{ 235 })  = e^{ 1233 }$

$d(e^{ 236 })  = (-1)e^{ 2233 }$

$d(e^{ 245 })  = e^{ 1225 } + (-1)e^{ 1234 }$

$d(e^{ 246 })  = e^{ 1226 } + e^{ 2234 }$

$d(e^{ 256 })  = e^{ 1236 } + e^{ 2235 }$

$d(e^{ 345 })  = (-1)e^{ 1235 } + (-1)e^{ 1334 }$

$d(e^{ 346 })  = (-1)e^{ 1236 } + (-1)e^{ 2334 }$

$d(e^{ 356 })  = e^{ 1336 } + (-1)e^{ 2335 }$

$d(e^{ 456 })  = e^{ 1256 } + (-1)e^{ 1346 } + e^{ 2345 }$

### Derivatives of $2-$forms
$d(e^{ 14 })  = (-1)e^{ 112 }$

$d(e^{ 15 })  = (-1)e^{ 113 }$

$d(e^{ 16 })  = (-1)e^{ 123 }$

$d(e^{ 24 })  = e^{ 122 }$

$d(e^{ 25 })  = e^{ 123 }$

$d(e^{ 26 })  = (-1)e^{ 223 }$

$d(e^{ 34 })  = (-1)e^{ 123 }$

$d(e^{ 35 })  = e^{ 133 }$

$d(e^{ 36 })  = e^{ 233 }$

$d(e^{ 45 })  = e^{ 125 } + (-1)e^{ 134 }$

$d(e^{ 46 })  = e^{ 126 } + (-1)e^{ 234 }$

$d(e^{ 56 })  = e^{ 136 } + (-1)e^{ 235 }$

### $d \Lambda d$ of $3-$forms
$d \Lambda d( e^{ 456 })  = (-3)e^{ 123 }$

\pagebreak

## Structure constants of the Lie Algebra:
$((-2)e^{ 15 }, \2e^{ 25 }, \(-2)e^{ 36 }, \2e^{ 46 }, \0, \0)$ 

### Symplectic form
 $\omega=e^{ 12 } + e^{ 34 } + e^{ 56 }$

### Derivatives of $3-$forms
$d(e^{ 123 })  = (-2)e^{ 1236 }$

$d(e^{ 124 })  = 2e^{ 1246 }$

$d(e^{ 134 })  = (-2)e^{ 1345 }$

$d(e^{ 135 })  = (-2)e^{ 1355 } + (-2)e^{ 1356 }$

$d(e^{ 136 })  = 2e^{ 1356 } + (-2)e^{ 1366 }$

$d(e^{ 145 })  = (-2)e^{ 1455 } + 2e^{ 1456 }$

$d(e^{ 146 })  = 2e^{ 1456 } + 2e^{ 1466 }$

$d(e^{ 156 })  = 2e^{ 1556 }$

$d(e^{ 234 })  = 2e^{ 2345 }$

$d(e^{ 235 })  = 2e^{ 2355 } + (-2)e^{ 2356 }$

$d(e^{ 236 })  = (-2)e^{ 2356 } + (-2)e^{ 2366 }$

$d(e^{ 245 })  = 2e^{ 2455 } + 2e^{ 2456 }$

$d(e^{ 246 })  = (-2)e^{ 2456 } + 2e^{ 2466 }$

$d(e^{ 256 })  = (-2)e^{ 2556 }$

$d(e^{ 356 })  = (-2)e^{ 3566 }$

$d(e^{ 456 })  = 2e^{ 4566 }$

### Derivatives of $2-$forms
$d(e^{ 13 })  = 2e^{ 135 } + 2e^{ 136 }$

$d(e^{ 14 })  = 2e^{ 145 } + (-2)e^{ 146 }$

$d(e^{ 15 })  = 2e^{ 155 }$

$d(e^{ 16 })  = (-2)e^{ 156 }$

$d(e^{ 23 })  = (-2)e^{ 235 } + 2e^{ 236 }$

$d(e^{ 24 })  = (-2)e^{ 245 } + (-2)e^{ 246 }$

$d(e^{ 25 })  = (-2)e^{ 255 }$

$d(e^{ 26 })  = 2e^{ 256 }$

$d(e^{ 35 })  = 2e^{ 356 }$

$d(e^{ 36 })  = 2e^{ 366 }$

$d(e^{ 45 })  = (-2)e^{ 456 }$

$d(e^{ 46 })  = (-2)e^{ 466 }$

### $d \Lambda d$ of $3-$forms
$d \Lambda d( e^{ 123 })  = (-4)e^{ 366 }$

$d \Lambda d( e^{ 124 })  = (-4)e^{ 466 }$

$d \Lambda d( e^{ 134 })  = (-4)e^{ 155 }$

$d \Lambda d( e^{ 135 })  = (-4)e^{ 135 } + (-4)e^{ 136 }$

$d \Lambda d( e^{ 136 })  = 4e^{ 135 } + 4e^{ 136 }$

$d \Lambda d( e^{ 145 })  = 4e^{ 145 } + (-4)e^{ 146 }$

$d \Lambda d( e^{ 146 })  = 4e^{ 145 } + (-4)e^{ 146 }$

$d \Lambda d( e^{ 156 })  = (-4)e^{ 155 }$

$d \Lambda d( e^{ 234 })  = (-4)e^{ 255 }$

$d \Lambda d( e^{ 235 })  = 4e^{ 235 } + (-4)e^{ 236 }$

$d \Lambda d( e^{ 236 })  = 4e^{ 235 } + (-4)e^{ 236 }$

$d \Lambda d( e^{ 245 })  = (-4)e^{ 245 } + (-4)e^{ 246 }$

$d \Lambda d( e^{ 246 })  = 4e^{ 245 } + 4e^{ 246 }$

$d \Lambda d( e^{ 256 })  = (-4)e^{ 255 }$

$d \Lambda d( e^{ 356 })  = (-4)e^{ 366 }$

$d \Lambda d( e^{ 456 })  = (-4)e^{ 466 }$

\pagebreak

## Structure constants of the Lie Algebra:
$(e^{ 23 }, \(-1)e^{ 36 }, \e^{ 26 }, \e^{ 26 } + (-1)e^{ 56 }, \e^{ 36 } + e^{ 46 }, \0)$ 

### Symplectic form
 $\omega=(-2)e^{ 16 } + (-1)e^{ 25 } + e^{ 34 }$

### Derivatives of $3-$forms
$d(e^{ 123 })  = e^{ 1226 } + e^{ 1336 } + (-1)e^{ 2233 }$

$d(e^{ 124 })  = e^{ 1226 } + (-1)e^{ 1256 } + (-1)e^{ 1346 } + e^{ 2234 }$

$d(e^{ 125 })  = e^{ 1236 } + e^{ 1246 } + (-1)e^{ 1356 } + e^{ 2235 }$

$d(e^{ 126 })  = (-1)e^{ 1366 } + e^{ 2236 }$

$d(e^{ 134 })  = (-1)e^{ 1236 } + e^{ 1246 } + (-1)e^{ 1356 } + (-1)e^{ 2334 }$

$d(e^{ 135 })  = e^{ 1256 } + e^{ 1336 } + e^{ 1346 } + (-1)e^{ 2335 }$

$d(e^{ 136 })  = e^{ 1266 } + (-1)e^{ 2336 }$

$d(e^{ 145 })  = e^{ 1256 } + (-1)e^{ 1346 } + e^{ 1446 } + e^{ 1556 } + e^{ 2345 }$

$d(e^{ 146 })  = e^{ 1266 } + (-1)e^{ 1566 } + e^{ 2346 }$

$d(e^{ 156 })  = e^{ 1366 } + e^{ 1466 } + e^{ 2356 }$

$d(e^{ 234 })  = (-1)e^{ 2236 } + e^{ 2246 } + (-1)e^{ 2356 } + e^{ 3346 }$

$d(e^{ 235 })  = e^{ 2256 } + e^{ 2336 } + e^{ 2346 } + e^{ 3356 }$

$d(e^{ 236 })  = e^{ 2266 } + e^{ 3366 }$

$d(e^{ 245 })  = e^{ 2256 } + (-1)e^{ 2346 } + e^{ 2446 } + e^{ 2556 } + (-1)e^{ 3456 }$

$d(e^{ 246 })  = e^{ 2266 } + (-1)e^{ 2566 } + (-1)e^{ 3466 }$

$d(e^{ 256 })  = e^{ 2366 } + e^{ 2466 } + (-1)e^{ 3566 }$

$d(e^{ 345 })  = (-1)e^{ 2356 } + e^{ 2456 } + (-1)e^{ 3346 } + e^{ 3446 } + e^{ 3556 }$

$d(e^{ 346 })  = (-1)e^{ 2366 } + e^{ 2466 } + (-1)e^{ 3566 }$

$d(e^{ 356 })  = e^{ 2566 } + e^{ 3366 } + e^{ 3466 }$

$d(e^{ 456 })  = e^{ 2566 } + (-1)e^{ 3466 } + e^{ 4466 } + e^{ 5566 }$

### Derivatives of $2-$forms
$d(e^{ 12 })  = e^{ 136 } + e^{ 223 }$

$d(e^{ 13 })  = (-1)e^{ 126 } + (-1)e^{ 233 }$

$d(e^{ 14 })  = (-1)e^{ 126 } + e^{ 156 } + e^{ 234 }$

$d(e^{ 15 })  = (-1)e^{ 136 } + (-1)e^{ 146 } + e^{ 235 }$

$d(e^{ 16 })  = e^{ 236 }$

$d(e^{ 23 })  = (-1)e^{ 226 } + (-1)e^{ 336 }$

$d(e^{ 24 })  = (-1)e^{ 226 } + e^{ 256 } + e^{ 346 }$

$d(e^{ 25 })  = (-1)e^{ 236 } + (-1)e^{ 246 } + e^{ 356 }$

$d(e^{ 26 })  = e^{ 366 }$

$d(e^{ 34 })  = e^{ 236 } + (-1)e^{ 246 } + e^{ 356 }$

$d(e^{ 35 })  = (-1)e^{ 256 } + (-1)e^{ 336 } + (-1)e^{ 346 }$

$d(e^{ 36 })  = (-1)e^{ 266 }$

$d(e^{ 45 })  = (-1)e^{ 256 } + e^{ 346 } + (-1)e^{ 446 } + (-1)e^{ 556 }$

$d(e^{ 46 })  = (-1)e^{ 266 } + e^{ 566 }$

$d(e^{ 56 })  = (-1)e^{ 366 } + (-1)e^{ 466 }$

### $d \Lambda d$ of $3-$forms
$d \Lambda d( e^{ 124 })  = (-1.5)e^{ 236 } + 2e^{ 246 } + (-2)e^{ 356 }$

$d \Lambda d( e^{ 125 })  = (-2.5)e^{ 226 } + 2e^{ 256 } + (-0.5)e^{ 336 } + 2e^{ 346 }$

$d \Lambda d( e^{ 126 })  = (-1)e^{ 266 }$

$d \Lambda d( e^{ 134 })  = (-1)e^{ 226 } + 2e^{ 256 } + e^{ 336 } + 2e^{ 346 }$

$d \Lambda d( e^{ 135 })  = 1.5e^{ 236 } + (-2)e^{ 246 } + 2e^{ 356 }$

$d \Lambda d( e^{ 136 })  = (-1)e^{ 366 }$

$d \Lambda d( e^{ 145 })  = (-3)e^{ 236 } + (-1.5)e^{ 246 } + 1.5e^{ 356 }$

$d \Lambda d( e^{ 146 })  = (-1)e^{ 366 } + (-1)e^{ 466 }$

$d \Lambda d( e^{ 156 })  = 2.5e^{ 266 } + (-1)e^{ 566 }$

$d \Lambda d( e^{ 234 })  = 0.5e^{ 266 }$

$d \Lambda d( e^{ 235 })  = 0.5e^{ 366 }$

$d \Lambda d( e^{ 245 })  = (-1)e^{ 366 } + 0.5e^{ 466 }$

$d \Lambda d( e^{ 345 })  = (-2)e^{ 266 } + 0.5e^{ 566 }$

\pagebreak

## Structure constants of the Lie Algebra:
$(e^{ 16 } + e^{ 35 }, \(-1)e^{ 26 } + e^{ 45 }, \e^{ 36 }, \(-1)e^{ 46 }, \0, \0)$ 

### Symplectic form
 $\omega=e^{ 14 } + e^{ 23 } + e^{ 56 }$

### Derivatives of $3-$forms
$d(e^{ 123 })  = e^{ 1236 } + (-1)e^{ 1345 } + e^{ 2335 }$

$d(e^{ 124 })  = (-1)e^{ 1246 } + (-1)e^{ 1445 } + (-1)e^{ 2345 }$

$d(e^{ 125 })  = e^{ 1455 } + (-1)e^{ 2355 }$

$d(e^{ 126 })  = (-1)e^{ 1456 } + e^{ 2356 }$

$d(e^{ 134 })  = e^{ 1346 } + (-1)e^{ 3345 }$

$d(e^{ 135 })  = 2e^{ 1356 } + (-1)e^{ 3355 }$

$d(e^{ 136 })  = 2e^{ 1366 } + e^{ 3356 }$

$d(e^{ 145 })  = e^{ 3455 }$

$d(e^{ 146 })  = (-1)e^{ 3456 }$

$d(e^{ 156 })  = e^{ 1566 } + (-1)e^{ 3556 }$

$d(e^{ 234 })  = (-1)e^{ 2346 } + e^{ 3445 }$

$d(e^{ 235 })  = (-1)e^{ 3455 }$

$d(e^{ 236 })  = e^{ 3456 }$

$d(e^{ 245 })  = (-2)e^{ 2456 } + (-1)e^{ 4455 }$

$d(e^{ 246 })  = (-2)e^{ 2466 } + e^{ 4456 }$

$d(e^{ 256 })  = (-1)e^{ 2566 } + (-1)e^{ 4556 }$

$d(e^{ 356 })  = e^{ 3566 }$

$d(e^{ 456 })  = (-1)e^{ 4566 }$

### Derivatives of $2-$forms
$d(e^{ 12 })  = (-1)e^{ 145 } + e^{ 235 }$

$d(e^{ 13 })  = (-2)e^{ 136 } + e^{ 335 }$

$d(e^{ 14 })  = (-1)e^{ 345 }$

$d(e^{ 15 })  = (-1)e^{ 156 } + (-1)e^{ 355 }$

$d(e^{ 16 })  = (-1)e^{ 166 } + e^{ 356 }$

$d(e^{ 23 })  = e^{ 345 }$

$d(e^{ 24 })  = 2e^{ 246 } + e^{ 445 }$

$d(e^{ 25 })  = e^{ 256 } + (-1)e^{ 455 }$

$d(e^{ 26 })  = e^{ 266 } + e^{ 456 }$

$d(e^{ 35 })  = (-1)e^{ 356 }$

$d(e^{ 36 })  = (-1)e^{ 366 }$

$d(e^{ 45 })  = e^{ 456 }$

$d(e^{ 46 })  = e^{ 466 }$

### $d \Lambda d$ of $3-$forms
$d \Lambda d( e^{ 123 })  = e^{ 166 } + e^{ 356 }$

$d \Lambda d( e^{ 124 })  = (-1)e^{ 266 } + e^{ 456 }$

$d \Lambda d( e^{ 126 })  = 2e^{ 345 }$

$d \Lambda d( e^{ 134 })  = (-1)e^{ 366 }$

$d \Lambda d( e^{ 135 })  = (-4)e^{ 136 } + 2e^{ 335 }$

$d \Lambda d( e^{ 156 })  = (-1)e^{ 166 }$

$d \Lambda d( e^{ 234 })  = e^{ 466 }$

$d \Lambda d( e^{ 245 })  = (-4)e^{ 246 } + (-2)e^{ 445 }$

$d \Lambda d( e^{ 256 })  = (-1)e^{ 266 }$

$d \Lambda d( e^{ 356 })  = (-1)e^{ 366 }$

$d \Lambda d( e^{ 456 })  = (-1)e^{ 466 }$

\pagebreak

