## Structure constants of the Lie Algebra:
$(0, 0)(0, 0)(0, 0)(15, 1)(0, 0)(13, 1)$

### Symplectic form
 $\omega=e^{ 12 } + e^{ 34 } + e^{ 56 }$

### Derivatives of $3-$forms
$d(e^{ 234 })  = e^{ 1235 }$

$d(e^{ 246 })  = (-1)e^{ 1234 } + e^{ 1256 }$

$d(e^{ 256 })  = (-1)e^{ 1235 }$

$d(e^{ 346 })  = e^{ 1356 }$

$d(e^{ 456 })  = e^{ 1345 }$

### Derivatives of $2-$forms
$d(e^{ 24 })  = e^{ 125 }$

$d(e^{ 26 })  = e^{ 123 }$

$d(e^{ 34 })  = e^{ 135 }$

$d(e^{ 46 })  = (-1)e^{ 134 } + e^{ 156 }$

$d(e^{ 56 })  = (-1)e^{ 135 }$

### $d \Lambda d$ of $3-$forms
$d \Lambda d( e^{ 246 })  = (-2)e^{ 135 }$

\pagebreak

## Structure constants of the Lie Algebra:
$(0, 0)(0, 0)(0, 0)(0, 0)(12, 1)(13, 1)$

### Symplectic form
 $\omega=(-1)e^{ 16 } + e^{ 25 } + e^{ 34 }$

### Derivatives of $3-$forms
$d(e^{ 246 })  = (-1)e^{ 1234 }$

$d(e^{ 256 })  = (-1)e^{ 1235 }$

$d(e^{ 345 })  = e^{ 1234 }$

$d(e^{ 356 })  = (-1)e^{ 1236 }$

$d(e^{ 456 })  = (-1)e^{ 1246 } + e^{ 1345 }$

### Derivatives of $2-$forms
$d(e^{ 26 })  = e^{ 123 }$

$d(e^{ 35 })  = (-1)e^{ 123 }$

$d(e^{ 45 })  = (-1)e^{ 124 }$

$d(e^{ 46 })  = (-1)e^{ 134 }$

$d(e^{ 56 })  = e^{ 126 } + (-1)e^{ 135 }$

### $d \Lambda d$ of $3-$forms
\pagebreak

## Structure constants of the Lie Algebra:
$(0, 0)(35, 1)(0, 0)(15, 0.5)(0, 0)(13, -0.5)$

### Symplectic form
 $\omega=e^{ 12 } + e^{ 34 } + e^{ 56 }$

### Derivatives of $3-$forms
$d(e^{ 124 })  = e^{ 1345 }$

$d(e^{ 126 })  = (-1)e^{ 1356 }$

$d(e^{ 234 })  = 0.5e^{ 1235 }$

$d(e^{ 246 })  = 0.5e^{ 1234 } + 0.5e^{ 1256 } + (-1)e^{ 3456 }$

$d(e^{ 256 })  = 0.5e^{ 1235 }$

$d(e^{ 346 })  = 0.5e^{ 1356 }$

$d(e^{ 456 })  = (-0.5)e^{ 1345 }$

### Derivatives of $2-$forms
$d(e^{ 12 })  = (-1)e^{ 135 }$

$d(e^{ 24 })  = 0.5e^{ 125 } + (-1)e^{ 345 }$

$d(e^{ 26 })  = (-0.5)e^{ 123 } + e^{ 356 }$

$d(e^{ 34 })  = 0.5e^{ 135 }$

$d(e^{ 46 })  = 0.5e^{ 134 } + 0.5e^{ 156 }$

$d(e^{ 56 })  = 0.5e^{ 135 }$

### $d \Lambda d$ of $3-$forms
$d \Lambda d( e^{ 246 })  = (-1.5)e^{ 135 }$

\pagebreak

## Structure constants of the Lie Algebra:
$(0, 0)(0, 0)(0, 0)(12, 1)(13, 1)(23, 1)$

### Symplectic form
 $\omega=2e^{ 16 } + e^{ 25 } + (-1)e^{ 34 }$

### Derivatives of $3-$forms
$d(e^{ 146 })  = e^{ 1234 }$

$d(e^{ 156 })  = e^{ 1235 }$

$d(e^{ 245 })  = (-1)e^{ 1234 }$

$d(e^{ 256 })  = e^{ 1236 }$

$d(e^{ 345 })  = (-1)e^{ 1235 }$

$d(e^{ 346 })  = (-1)e^{ 1236 }$

$d(e^{ 456 })  = e^{ 1256 } + (-1)e^{ 1346 } + e^{ 2345 }$

### Derivatives of $2-$forms
$d(e^{ 16 })  = (-1)e^{ 123 }$

$d(e^{ 25 })  = e^{ 123 }$

$d(e^{ 34 })  = (-1)e^{ 123 }$

$d(e^{ 45 })  = e^{ 125 } + (-1)e^{ 134 }$

$d(e^{ 46 })  = e^{ 126 } + (-1)e^{ 234 }$

$d(e^{ 56 })  = e^{ 136 } + (-1)e^{ 235 }$

### $d \Lambda d$ of $3-$forms
$d \Lambda d( e^{ 456 })  = (-3)e^{ 123 }$

\pagebreak

## Structure constants of the Lie Algebra:
$(15, -2)(25, 2)(36, -2)(46, 2)(0, 0)(0, 0)$

### Symplectic form
 $\omega=e^{ 12 } + e^{ 34 } + e^{ 56 }$

### Derivatives of $3-$forms
$d(e^{ 123 })  = (-2)e^{ 1236 }$

$d(e^{ 124 })  = 2e^{ 1246 }$

$d(e^{ 134 })  = (-2)e^{ 1345 }$

$d(e^{ 135 })  = (-2)e^{ 1356 }$

$d(e^{ 136 })  = 2e^{ 1356 }$

$d(e^{ 145 })  = 2e^{ 1456 }$

$d(e^{ 146 })  = 2e^{ 1456 }$

$d(e^{ 234 })  = 2e^{ 2345 }$

$d(e^{ 235 })  = (-2)e^{ 2356 }$

$d(e^{ 236 })  = (-2)e^{ 2356 }$

$d(e^{ 245 })  = 2e^{ 2456 }$

$d(e^{ 246 })  = (-2)e^{ 2456 }$

### Derivatives of $2-$forms
$d(e^{ 13 })  = 2e^{ 135 } + 2e^{ 136 }$

$d(e^{ 14 })  = 2e^{ 145 } + (-2)e^{ 146 }$

$d(e^{ 16 })  = (-2)e^{ 156 }$

$d(e^{ 23 })  = (-2)e^{ 235 } + 2e^{ 236 }$

$d(e^{ 24 })  = (-2)e^{ 245 } + (-2)e^{ 246 }$

$d(e^{ 26 })  = 2e^{ 256 }$

$d(e^{ 35 })  = 2e^{ 356 }$

$d(e^{ 45 })  = (-2)e^{ 456 }$

### $d \Lambda d$ of $3-$forms
$d \Lambda d( e^{ 135 })  = (-4)e^{ 135 } + (-4)e^{ 136 }$

$d \Lambda d( e^{ 136 })  = 4e^{ 135 } + 4e^{ 136 }$

$d \Lambda d( e^{ 145 })  = 4e^{ 145 } + (-4)e^{ 146 }$

$d \Lambda d( e^{ 146 })  = 4e^{ 145 } + (-4)e^{ 146 }$

$d \Lambda d( e^{ 235 })  = 4e^{ 235 } + (-4)e^{ 236 }$

$d \Lambda d( e^{ 236 })  = 4e^{ 235 } + (-4)e^{ 236 }$

$d \Lambda d( e^{ 245 })  = (-4)e^{ 245 } + (-4)e^{ 246 }$

$d \Lambda d( e^{ 246 })  = 4e^{ 245 } + 4e^{ 246 }$

\pagebreak

